theories/VRcomp.v
@@ -1,0 +1,283 @@
+From Coq Require Import Arith.
+From Coq Require Import Lists.List.
+Import ListNotations.
+From Coq Require Import Lia.
+From Coq Require Import Classes.EquivDec.
+
+From Peg Require Import Syntax.
+From Peg Require Import NMatch.
+From Peg Require Import NVerifyrule.
+
+
+Fixpoint verifyrule_comp gas
+    (g : grammar) (p : pat) (lr : list RuleStatus) (nb : bool) :
+      option Result :=
+  match gas with
+  | 0 => None
+  | S gas' =>
+    match p with
+    | PEmpty => Some (Some (true, lr))
+    | PSet _ => Some (Some (nb, lr))
+    | PSequence p1 p2 =>
+      match verifyrule_comp gas' g p1 lr false with
+      | None => None  (* out of gas *)
+      | Some None => Some None  (* ill formed *)
+      | Some (Some (false, lr')) => Some (Some (nb, lr'))
+      | Some (Some (true, lr')) => verifyrule_comp gas' g p2 lr' nb
+      end
+    | PChoice p1 p2 =>
+      match verifyrule_comp gas' g p1 lr nb with
+      | None => None  (* out of gas *)
+      | Some None => Some None  (* ill formed *)
+      | Some (Some (nb', lr')) => verifyrule_comp gas' g p2 lr' nb'
+      end
+    | PRepetition p' => verifyrule_comp gas' g p' lr true
+    | PNot p' => verifyrule_comp gas' g p' lr true
+    | PAnd p' => verifyrule_comp gas' g p' lr true
+    | PNT i =>
+      match nth i lr Visiting with
+      | Visiting => Some (None)  (* ill formed *)
+      | Visited nb' => Some (Some (orb nb nb', lr))
+      | NotVisited =>
+        match verifyrule_comp gas' g (nth i g PEmpty)
+                              (update lr i Visiting) false with
+        | None => None  (* out of gas *)
+        | Some None => Some None  (* ill formed *)
+        | Some (Some (nb', lr')) =>
+            Some (Some (orb nb nb', update lr' i (Visited nb')))
+        end
+      end
+    end
+  end.
+
+
+Ltac destVR :=
+  match goal with
+  | [H: context [verifyrule_comp ?gas ?g ?p1 ?lr ?nb] |- _]
+        => destruct (verifyrule_comp gas g p1 lr nb) as [[[? ?] | ] | ] eqn:Heq
+  | [|- context [verifyrule_comp ?gas ?g ?p1 ?lr ?nb]]
+        => destruct (verifyrule_comp gas g p1 lr nb) as [[[? ?] | ] | ] eqn:Heq
+  end.
+
+
+Lemma verifyrule_comp_sound : forall gas g p lr nb res,
+  verifyrule_comp gas g p lr nb = Some res ->
+  verifyrule g p lr nb res.
+Proof with eauto using verifyrule.
+  induction gas; intros * H; try discriminate.
+  destruct p; simpl in H;
+    try (injection H; intros; subst);
+      try discriminate...
+  - destVR; try discriminate; simplsome...
+    destruct b; simplsome...
+  - destVR; simplsome...
+  - destruct (nth n lr Visiting) eqn:?; simplsome...
+    destVR; simplsome...
+Qed.
+
+
+Ltac breakEx :=
+  repeat match goal with
+  [H: exists _, _ |- _] => destruct H as [? ?]
+  end.
+
+Lemma verifyrule_comp_gas_exists : forall g p lr nb res,
+    verifyrule g p lr nb res ->
+    exists gas,
+      forall gas', gas < gas' -> verifyrule_comp gas' g p lr nb = Some res.
+Proof.
+  induction 1; intros *;
+    try (exists 0; destruct gas'; try lia; trivial; fail);
+    try (breakEx; exists (S x); intros * Hlt;
+    destruct gas'; try lia; simpl;
+    apply H0; lia; fail).
+  - breakEx. exists (S x). intros * Hlt.
+    destruct gas'. try lia. simpl.
+    rewrite H0; trivial; lia.
+  - breakEx. exists (S (x + x0)).
+    destruct gas'; try lia. simpl.
+    intros Hlt. rewrite H2; try lia; rewrite H1; trivial; lia.
+  - breakEx. exists (S x).
+    intros * Htl.
+    destruct gas'; try lia. simpl.
+    rewrite H0; trivial; try lia.
+  - breakEx. exists (S x).
+    destruct gas'; try lia; simpl.
+    intros ?. rewrite H0; trivial; try lia.
+  - breakEx. exists (S (x + x0)).
+    destruct gas'; try lia; simpl.
+    intros ?. rewrite H2; try lia.
+    apply H1; lia.
+  - exists 1. intros gas' Hlt.
+    destruct gas'; try lia; simpl.
+    rewrite H; trivial.
+  - breakEx. exists (S x). intros gas' Hlt.
+    destruct gas'; try lia; simpl.
+    rewrite H. subst.
+    rewrite H2; trivial; lia.
+  - breakEx. exists (S x). subst.
+    intros gas' Hlt.
+    destruct gas'; try lia; simpl.
+    rewrite H.
+    rewrite H2; trivial; try lia.
+  - exists 1; intros gas' Hlt.
+    destruct gas'; try lia; simpl.
+    rewrite H. trivial.
+Qed.
+
+
+Fixpoint costP p : nat :=
+  match p with
+  | PEmpty => 1
+  | PSet _ => 1
+  | PSequence p1 p2 => S (costP p1 + costP p2)
+  | PChoice p1 p2 => S (costP p1 + costP p2)
+  | PRepetition p => S (costP p)
+  | PNot p => S (costP p)
+  | PAnd p => S (costP p)
+  | PNT _ => 1
+  end.
+
+
+Lemma costP1 : forall p, 0 < costP p.
+Proof. induction p; simpl; lia. Qed.
+
+
+Fixpoint costG g lr : nat :=
+  match lr with
+  | nil => 0
+  | NotVisited :: lr' =>
+      match g with
+      | nil => S (1 + costG nil lr')
+      | (p :: g') => S (costP p + costG g' lr')
+      end
+  | _ :: lr' =>
+      match g with
+      | nil => costG nil lr'
+      | (_ :: g') => costG g' lr'
+      end
+  end.
+
+
+Lemma CostUpdateVIsitingP : forall lr g n,
+    nth n lr Visiting = NotVisited ->
+    costP (nth n g PEmpty) + costG g (update lr n Visiting) <= costG g lr.
+Proof.
+  induction lr; intros * Hn.
+  - simpl in Hn. destruct n; discriminate.
+  - simpl. destruct n; destruct a; destruct g; simpl; try lia;
+     try discriminate; simpl in Hn;
+     try (apply IHlr with (g := g) in Hn; simpl in Hn; lia);
+     try (apply IHlr with (g := nil) in Hn; destruct n; simpl in Hn; lia).
+Qed.
+
+
+Lemma costUpdateVisited : forall lr g i nb,
+  costG g (update lr i (Visited nb)) <= costG g lr.
+Proof.
+  induction lr; intros *.
+  - simpl. destruct i; trivial.
+  - destruct g.
+    + simpl. destruct i; simpl.
+      * simpl. destruct a; lia.
+      * simpl. destruct a; specialize (IHlr nil i nb) as ?; lia.
+    + simpl. destruct i; simpl; destruct a; try lia;
+      specialize (IHlr g i nb) as ?; lia.
+Qed.
+
+
+Lemma costUpdateVisiting : forall lr g i,
+  costG g (update lr i Visiting) <= costG g lr.
+Proof.
+  induction lr; intros *.
+  - simpl. destruct i; trivial.
+  - destruct g.
+    + simpl. destruct i; simpl.
+      * simpl. destruct a; lia.
+      * simpl. destruct a; specialize (IHlr nil i) as ?; lia.
+    + simpl. destruct i; simpl; destruct a; try lia;
+      specialize (IHlr g i) as ?; lia.
+Qed.
+
+
+Lemma dimCost : forall gas g p lr lr' nb nb',
+    verifyrule_comp gas g p lr nb = Some (Some (nb', lr')) ->
+    costG g lr' <= costG g lr.
+Proof.
+  induction gas; intros * HVr; try discriminate.
+  destruct p; simpl in HVr; simplsome; trivial;
+    repeat match goal with
+    [H : verifyrule_comp _ _ _ _ _ = Some _ |- _] =>
+       eapply IHgas in H
+    end; try lia.
+  - destVR; try congruence.
+    destruct b.
+    + eapply IHgas in Heq.
+      eapply IHgas in HVr.
+      lia.
+    + simplsome.
+      eapply IHgas in Heq.
+      trivial.
+  - destVR; try congruence.
+    eapply IHgas in Heq.
+    eapply IHgas in HVr.
+    lia.
+  - destruct (nth n lr Visiting); try congruence.
+    + destVR; try congruence.
+      simplsome.
+      apply IHgas in Heq; clear IHgas.
+      specialize (costUpdateVisited l g n b) as ?.
+      specialize (costUpdateVisiting lr g n) as ?.
+      lia.
+    + simplsome. trivial.
+Qed.
+
+
+Lemma VR_comp : forall gas g p lr nb,
+    (costG g lr + costP p) <= gas ->
+    verifyrule_comp gas g p lr nb <> None.
+Proof.
+  induction gas; intros * Hle.
+  - specialize (costP1 p). lia.
+  - destruct p.
+    + simpl. congruence.
+    + simpl. congruence.
+    + simpl in Hle; simpl.
+      destVR; try congruence.
+      destruct b; try congruence.
+      * eapply IHgas.
+        eapply dimCost in Heq. lia.
+      * exfalso. eapply IHgas; eauto. lia.
+    + simpl in Hle; simpl.
+      destVR; try congruence.
+      * eapply IHgas.
+        apply dimCost in Heq. lia.
+      * exfalso. eapply IHgas; eauto. lia.
+    + apply IHgas. simpl in Hle. lia.
+    + apply IHgas. simpl in Hle. lia.
+    + apply IHgas. simpl in Hle. lia.
+    + simpl in Hle; simpl.
+      destruct (nth n lr Visiting) eqn:?; try congruence.
+      destVR; try congruence.
+      exfalso.
+      eapply IHgas; eauto.
+      specialize (CostUpdateVIsitingP lr g n Heqr) as ?.
+      lia.
+Qed.
+
+
+Lemma VRVR : forall g p lr nb res,
+  verifyrule_comp (S (costG g lr + costP p)) g p lr nb = Some res <->
+  verifyrule g p lr nb res.
+Proof.
+  intros *; split; intro H.
+  - eauto using verifyrule_comp_sound.
+  - assert (H1 : costG g lr + costP p <= S (costG g lr + costP p)) by lia.
+    specialize (VR_comp (S (costG g lr + costP p)) g p lr nb H1) as H2.
+    destruct (verifyrule_comp (S (costG g lr + costP p)) g p lr nb) eqn:?.
+    + apply verifyrule_comp_sound in Heqo.
+      f_equal. eauto using verifyrule_unique.
+    + exfalso. apply H2. trivial.
+Qed.
+
+
